updates

Veritas.Verifier.EAC.fst
@@ -14,17 +14,6 @@ open Veritas.State
 open Veritas.Verifier
 open Veritas.Verifier.CorrectDefs
 
-(* the eac state of a key after processing an eac_log *)
-let eac_state_key (le: vlog_ext) (k:key): eac_state = 
-  let lek = partn eac_sm k le in
-  seq_machine_run eac_smk lek
-
-(* the state of a verifier thread after processing entries in a log *)
-let verifier_thread_state (#n:nat) (itsl: its_log n) (id:nat{id < n}): (st:vtls{Valid? st}) = 
-  let gl = partition_idx_seq itsl in
-  assert(t_verifiable (index (attach_index gl) id));
-  t_verify id (index gl id)
-
 (* generalized single- and multi-set hash collision *)
 type hash_collision_gen =
   | SingleHashCollision: hc: hash_collision -> hash_collision_gen
@@ -34,47 +23,95 @@ type hash_collision_gen =
 let hash_collision_contra (_:unit{False}): hash_collision_gen = 
   SingleHashCollision (Collision (DVal Null) (DVal Null))
 
+(* the eac state of a key after processing an eac_log *)
+let eac_state_key (le: vlog_ext) (k:key): eac_state = 
+  let lek = partn eac_sm k le in
+  seq_machine_run eac_smk lek
+
+(* the eac state of a key at the end of an its log *)
+let eac_state_of_key (#n:nat) (itsl: its_log n) (k:key): eac_state = 
+  let tsle = time_seq_ext itsl in 
+  let tslek = partn eac_sm k tsle in
+  seq_machine_run eac_smk tslek
+
+(* is the eac state of key at the end of its_log init *)
+let is_eac_state_init (#n:nat) (itsl: its_log n) (k:key): bool =
+  eac_state_of_key itsl k = EACInit
+
+(* is the key k in evicted state in *)
+let is_eac_state_evicted (#n:nat) (itsl: its_log n) (k:key): bool = 
+  EACEvicted? (eac_state_of_key itsl k)
+
+(* is the key k in instore state after processing its_log *)
+let is_eac_state_instore (#n:nat) (itsl: its_log n) (k:key):bool = 
+  EACInStore? (eac_state_of_key itsl k)
+
+(* the state of a verifier thread after processing entries in a log *)
+let verifier_thread_state (#n:nat) (itsl: its_log n) (id:nat{id < n}): (st:vtls{Valid? st}) = 
+  let gl = partition_idx_seq itsl in
+  assert(t_verifiable (index (attach_index gl) id));
+  t_verify id (index gl id)
+
 (* 
  * when the eac state of a key is Init (no operations on the key yet) no 
  * thread contains the key in its store 
  *)
 let lemma_eac_state_init_store 
    (#n:nat) 
-   (itsl: its_log n) (k: key{k <> Root /\ 
-                             EACInit = eac_state_key (time_seq_ext itsl) k}) (id:nat{id < n}):
+   (itsl: eac_ts_log n) (k: key{k <> Root && is_eac_state_init itsl k}) (id:nat{id < n}):
    Lemma (not (store_contains (thread_store (verifier_thread_state itsl id)) k)) 
    = admit()
 
 (* when the eac state of a key is EACEvicted then no thread contains the key in its store *)
-let lemma_eac_state_evicted_store (#n:nat) (itsl: its_log n) 
-  (k: key{EACEvicted? (eac_state_key (time_seq_ext itsl) k)}) (id:nat{id < n}):
+let lemma_eac_state_evicted_store (#n:nat) (itsl: eac_ts_log n) 
+  (k: key{is_eac_state_evicted itsl k}) (id:nat{id < n}):
     Lemma (not (store_contains (thread_store (verifier_thread_state itsl id)) k)) = admit()
 
-(* when the eac state of a key is EACInCache return the index of the last add that transitioned
- * the key k to "in cache" *)
-let last_add_idx (#n:nat) (itsl: its_log n)
-  (k: key{EACInCache? (eac_state_key (time_seq_ext itsl) k)}): seq_index itsl =
-    admit()
+(* does a log have some add entry *)
+let has_some_add (l:seq vlog_entry): bool = 
+  exists_sat_elems is_add l
+
+(* does a log have some add of key k *)
+let has_some_add_of_key (k:key) (l:seq vlog_entry): bool = 
+  exists_sat_elems (is_add_of_key k) l 
+  
+(* when the eac state of a key is "instore" then there is always a previous add *)
+let lemma_eac_state_instore_implies_prev_add (#n:nat) (itsl: eac_ts_log n) (k:key{is_eac_state_instore itsl k}):
+  Lemma (has_some_add_of_key k (project_seq itsl)) = admit()
+
+(* when the eac state of a key is instore return the index of the last add that transitioned
+ * the key k to "instore" *)
+let last_add_idx (#n:nat) (itsl: eac_ts_log n) (k: key{is_eac_state_instore itsl k}): seq_index itsl =
+   lemma_eac_state_instore_implies_prev_add itsl k;
+   last_index (is_add_of_key k) (project_seq itsl)
+
+(* the verifier thread where the last add of key k happens *)
+let last_add_tid (#n:nat) (itsl: eac_ts_log n) (k: key{is_eac_state_instore itsl k}): (tid:nat{tid < n}) =
+  snd (index itsl (last_add_idx itsl k))
+
+(* if the eac_state of k is instore, then that k is in the store of the verifier thread of its last add *)
+let lemma_eac_state_instore (#n:nat) (itsl: eac_ts_log n) (k:key{is_eac_state_instore itsl k}):
+  Lemma (store_contains (thread_store (verifier_thread_state itsl (last_add_tid itsl k))) k) = admit()
 
 (* the entry that causes the eac_invalidation *)
-let invalidating_log_entry (#n:nat) (itsl: non_eac_ts_log #n): vlog_entry_ext = 
+let invalidating_log_entry (#n:nat) (itsl: non_eac_ts_log n): vlog_entry_ext = 
   let tsle = time_seq_ext itsl in  
   let i = max_eac_prefix tsle in  
   index tsle i
 
 (* the key that causes the eac_invalidation *)
-let eac_invalidating_key (#n:nat) (itsl: non_eac_ts_log #n): key =
+let eac_invalidating_key (#n:nat) (itsl: non_eac_ts_log n): key =
   vlog_entry_ext_key (invalidating_log_entry itsl)
 
 (* last valid eac state *)
-let last_valid_eac_state (#n:nat) (itsl: non_eac_ts_log #n): eac_state = 
+let last_valid_eac_state (#n:nat) (itsl: non_eac_ts_log n): eac_state = 
   let tsle = time_seq_ext itsl in  
   let i = max_eac_prefix tsle in
   let k = eac_invalidating_key itsl in
   eac_state_key (prefix tsle i) k
   
 (* applying the invalidating entry on the last valid state produces EAC failure *)
-let lemma_invalidation (#n:nat) (itsl: non_eac_ts_log #n):
+let lemma_invalidation (#n:nat) (itsl: non_eac_ts_log n):
   Lemma (EACFail <> last_valid_eac_state itsl /\
          EACFail = eac_add (invalidating_log_entry itsl) (last_valid_eac_state itsl)) =            
   let tsl = project_seq itsl in
@@ -147,10 +184,10 @@ let lemma_time_seq_ext_correct (#n:nat) (itsl: its_log n) (i:seq_index itsl):
         [SMTPat (to_vlog_entry (index (time_seq_ext itsl) i))] =
   lemma_unzip_index itsl i
 
-(* if an operation requires the key in cache, it cannot be the first operation *)
-let lemma_non_eac_init_requires_key_in_cache (#n:nat) 
-  (itsl: non_eac_ts_log #n{last_valid_eac_state itsl = EACInit /\
-                           requires_key_in_cache (to_vlog_entry (invalidating_log_entry itsl)) /\
+(* if an operation requires the key in store, it cannot be the first operation *)
+let lemma_non_eac_init_requires_key_in_store (#n:nat) 
+  (itsl: non_eac_ts_log n{last_valid_eac_state itsl = EACInit /\
+                           requires_key_in_store (to_vlog_entry (invalidating_log_entry itsl)) /\
                            Root <> vlog_entry_key (to_vlog_entry (invalidating_log_entry itsl))}):  
   hash_collision_gen = 
   let tsle = time_seq_ext itsl in
@@ -169,8 +206,8 @@ let lemma_non_eac_init_requires_key_in_cache (#n:nat)
 
 (* the first operation for a key cannot be evict *)
 let lemma_non_eac_init_evict (#n:nat)
-  (itsl: non_eac_ts_log #n{last_valid_eac_state itsl = EACInit /\
-                           requires_key_in_cache (to_vlog_entry (invalidating_log_entry itsl)) /\
+  (itsl: non_eac_ts_log n{last_valid_eac_state itsl = EACInit /\
+                           requires_key_in_store (to_vlog_entry (invalidating_log_entry itsl)) /\
                            is_evict (to_vlog_entry (invalidating_log_entry itsl))}): hash_collision_gen =
   let tsle = time_seq_ext itsl in
   let i = max_eac_prefix tsle in
@@ -185,25 +222,25 @@ let lemma_non_eac_init_evict (#n:nat)
   let k = vlog_entry_key e in
   lemma_root_never_evicted (verifier_thread_state itsli tid) e;  
   assert(k <> Root);                               
-  lemma_non_eac_init_requires_key_in_cache itsl
+  lemma_non_eac_init_requires_key_in_store itsl
 
 (* the first operation for a key cannot be a blum add *)
 let lemma_non_eac_init_addb (#n)
-  (itsl: non_eac_ts_log #n{last_valid_eac_state itsl = EACInit /\
+  (itsl: non_eac_ts_log n{last_valid_eac_state itsl = EACInit /\
                            AddB? (to_vlog_entry (invalidating_log_entry itsl))}): hash_collision_gen =
   admit()                           
 
-let lemma_non_eac_time_seq_implies_hash_collision (#n:nat) (itsl: non_eac_ts_log #n): hash_collision_gen = 
+let lemma_non_eac_time_seq_implies_hash_collision (#n:nat) (itsl: non_eac_ts_log n): hash_collision_gen = 
   let st = last_valid_eac_state itsl in
   let ee = invalidating_log_entry itsl in
   match st with
   | EACInit -> (
       match ee with 
-      | NEvict (Get _ _) -> lemma_non_eac_init_requires_key_in_cache itsl
-      | NEvict (Put _ _) -> lemma_non_eac_init_requires_key_in_cache itsl
+      | NEvict (Get _ _) -> lemma_non_eac_init_requires_key_in_store itsl
+      | NEvict (Put _ _) -> lemma_non_eac_init_requires_key_in_store itsl
       | NEvict (AddB _ _ _) -> lemma_non_eac_init_addb itsl
       | Evict (EvictM _ _) _ -> lemma_non_eac_init_evict itsl
       | _ -> admit()
     )
-  | EACInCache m v -> admit()
+  | EACInStore m v -> admit()
   | EACEvicted m v -> admit()
