Veritas.Verifier.CorrectDefs.fst
@@ -155,7 +155,7 @@ let lemma_time_seq_correct (gl: g_verifiable_log)
   Lemma (g_entry_time gl (time_seq_source gl i) `ts_leq` g_entry_time gl (time_seq_source gl j))
   = admit()
 
-let requires_key_in_cache (e:vlog_entry): bool = 
+let requires_key_in_store (e:vlog_entry): bool = 
   match e with
   | Get _ _ -> true
   | Put _ _ -> true
@@ -164,7 +164,7 @@ let requires_key_in_cache (e:vlog_entry): bool =
   | EvictBM _ _ _ -> true
   | _ -> false
 
-let lemma_requires_key_in_cache (st: vtls) (e:vlog_entry{requires_key_in_cache e && 
+let lemma_requires_key_in_store (st: vtls) (e:vlog_entry{requires_key_in_store e && 
                                                          Valid? (t_verify_step st e)}):
   Lemma (Valid? st && store_contains (thread_store st) (vlog_entry_key e)) = 
   ()
@@ -276,5 +276,5 @@ let lemma_its_prefix_ext (#n:nat) (itsl:its_log n) (i:nat{i <= length itsl}):
         [SMTPat (time_seq_ext (its_prefix itsl i))] = 
   admit()
 
-type eac_ts_log (#n:nat) = itsl: its_log n {is_eac_log (time_seq_ext itsl)}
-type non_eac_ts_log (#n:nat) = itsl: its_log n {not (is_eac_log (time_seq_ext itsl))}
+type eac_ts_log (n:nat) = itsl: its_log n {is_eac_log (time_seq_ext itsl)}
+type non_eac_ts_log (n:nat) = itsl: its_log n {not (is_eac_log (time_seq_ext itsl))}
